ccc26x86/Asm_eff.v
@@ -99,9 +99,134 @@ End CEVAL_BUILTIN_ARG_COMPUTE.
 
 Section EFFSEM.
 
+Definition effect_instr (ge:genv) (c: code) (i: instruction) (rs: regset) (m: mem) 
+           : (block -> Z -> bool)  :=
+  match i with
+  (** Moves *)(*
+  | Pmov_rr rd r1 => EmptyEffect
+  | Pmov_ri rd n => EmptyEffect
+  | Pmov_ra rd id => EmptyEffect
+  | Pmov_rm rd a => EmptyEffect*)
+  | Pfstps_m a => (StoreEffect (eval_addrmode ge a rs) (encode_val Mfloat32 (rs ST0)))
+(*      exec_store Mfloat32 m a rs ST0 (ST0 :: nil)*)
+
+  | Pfstpl_m a => (StoreEffect (eval_addrmode ge a rs) (encode_val Mfloat64 (rs ST0)))
+(*      exec_store Mfloat64 m a rs ST0 (ST0 :: nil)*)
+
+  | Pmovss_mf a r1 => (StoreEffect (eval_addrmode ge a rs) (encode_val Mfloat32 (rs r1)))
+(*      exec_store Mfloat32 m a rs r1 nil*)
+
+  | Pmov_mr a r1 => (StoreEffect (eval_addrmode ge a rs) (encode_val Mint32 (rs r1)))
+  | Pmov_mr_a a r1 => (StoreEffect (eval_addrmode ge a rs) (encode_val Many32 (rs r1)))
+(*  | Pmovsd_ff rd r1 => EmptyEffect
+  | Pmovsd_fi rd n => EmptyEffect
+  | Pmovsd_fm rd a => EmptyEffect*)
+  | Pmovsd_mf a r1 => (StoreEffect (eval_addrmode ge a rs) (encode_val Mfloat64 (rs r1)))
+  | Pmovsd_mf_a a r1 => (StoreEffect (eval_addrmode ge a rs) (encode_val Many64 (rs r1)))
+(*  | Pfld_f r1 => EmptyEffect
+  | Pfld_m a => EmptyEffect
+  | Pfstp_f rd => EmptyEffect*)
+(*  | Pfstp_m a => StoreEffect (eval_addrmode ge a rs) (encode_val Mfloat64(*al32*) (rs ST0))*)
+(*  | Pxchg_rr r1 r2 => EmptyEffect*)
+
+  (** Moves with conversion *)
+  | Pmovb_mr a r1 => StoreEffect (eval_addrmode ge a rs) (encode_val Mint8unsigned (rs r1))
+  | Pmovw_mr a r1 => StoreEffect (eval_addrmode ge a rs) (encode_val Mint16unsigned (rs r1))
+(*  | Pmovzb_rr rd r1 => EmptyEffect
+  | Pmovzb_rm rd a => EmptyEffect
+  | Pmovsb_rr rd r1 => EmptyEffect
+  | Pmovsb_rm rd a => EmptyEffect
+  | Pmovzw_rr rd r1 => EmptyEffect
+  | Pmovzw_rm rd a => EmptyEffect
+  | Pmovsw_rr rd r1 => EmptyEffect
+  | Pmovsw_rm rd a => EmptyEffect
+  | Pcvtss2sd_fm rd a => EmptyEffect
+  | Pcvtsd2ss_ff rd r1 => EmptyEffect*)
+(*  | Pcvtsd2ss_mf a r1 => StoreEffect (eval_addrmode ge a rs) (encode_val Mfloat32 (rs r1))*)
+(*  | Pcvttsd2si_rf rd r1 => EmptyEffect
+  | Pcvtsi2sd_fr rd r1 => EmptyEffect*)
+
+  (** Integer arithmetic *)
+(*  | Plea rd a => EmptyEffect
+  | Pneg rd => EmptyEffect
+  | Psub_rr rd r1 => EmptyEffect
+  | Pimul_rr rd r1 => EmptyEffect
+  | Pimul_ri rd n => EmptyEffect
+  | Pimul_r r1 => EmptyEffect
+  | Pmul_r r1 => EmptyEffect
+  | Pdiv r1 =>  EmptyEffect
+  | Pidiv r1 => EmptyEffect
+  | Pand_rr rd r1 => EmptyEffect
+  | Pand_ri rd n => EmptyEffect
+  | Por_rr rd r1 => EmptyEffect
+  | Por_ri rd n => EmptyEffect
+  | Pxor_r rd => EmptyEffect
+  | Pxor_rr rd r1 => EmptyEffect
+  | Pxor_ri rd n => EmptyEffect
+  | Psal_rcl rd => EmptyEffect
+  | Psal_ri rd n => EmptyEffect
+  | Pshr_rcl rd => EmptyEffect
+  | Pshr_ri rd n => EmptyEffect
+  | Psar_rcl rd => EmptyEffect
+  | Psar_ri rd n => EmptyEffect
+  | Pshld_ri rd r1 n => EmptyEffect
+  | Pror_ri rd n => EmptyEffect
+  | Pcmp_rr r1 r2 => EmptyEffect
+  | Pcmp_ri r1 n => EmptyEffect
+  | Ptest_rr r1 r2 => EmptyEffect
+  | Ptest_ri r1 n => EmptyEffect
+  | Pcmov c rd r1 => EmptyEffect
+  | Psetcc c rd => EmptyEffect*)
+
+  (** Arithmetic operations over floats *)
+(*  | Paddd_ff rd r1 => EmptyEffect
+  | Psubd_ff rd r1 => EmptyEffect
+  | Pmuld_ff rd r1 => EmptyEffect
+  | Pdivd_ff rd r1 => EmptyEffect
+  | Pnegd rd => EmptyEffect
+  | Pabsd rd => EmptyEffect
+  | Pcomisd_ff r1 r2 => EmptyEffect
+  | Pxorpd_f rd => EmptyEffect*)
+
+  (** Branches and calls *)
+(*  | Pjmp_l lbl => EmptyEffect
+  | Pjmp_s id => EmptyEffect
+  | Pjmp_r r => EmptyEffect
+  | Pjcc cond lbl => EmptyEffect
+  | Pjcc2 cond1 cond2 lbl => EmptyEffect
+  | Pjmptbl r tbl => EmptyEffect
+  | Pcall_s id => EmptyEffect
+  | Pcall_r r => EmptyEffect
+  | Pret => EmptyEffect*)
+  (** Pseudo-instructions *)
+(*  | Plabel lbl => EmptyEffect
+  | Pallocframe sz ofs_ra ofs_link => EmptyEffect*)
+  | Pfreeframe sz ofs_ra ofs_link =>
+      match Mem.loadv Mint32 m (Val.add rs#ESP (Vint ofs_ra)) with
+      | None => EmptyEffect 
+      | Some ra =>
+          match Mem.loadv Mint32 m (Val.add rs#ESP (Vint ofs_link)) with
+          | None => EmptyEffect 
+          | Some sp =>
+              match rs#ESP with
+              | Vptr stk ofs =>
+                  match Mem.free m stk 0 sz with
+                  | None => EmptyEffect
+                  | Some m' => (FreeEffect m 0 sz stk) 
+                  end
+              | _ => EmptyEffect
+              end
+          end
+      end
+  | Pbuiltin ef args res => EmptyEffect
+(*     (BuiltinEffect ge ef (decode_longs (sig_args (ef_sig ef)) (map rs args)) m)*)
+(*  | Pannot ef args =>
+      EmptyEffect *)
+  | _ => EmptyEffect
+  end. (*
 Definition effect_instr (ge:genv) (c: code) (i: instruction) 
                  (rs: regset) (m: mem)
-           : (block -> Z -> bool)  := EmptyEffect.
+           : (block -> Z -> bool)  := EmptyEffect.*)
 (*
 Definition effect_instr (ge:genv) (e: preg -> val) (sp:val) (*(c: code)*) (i: instruction) 
                  (*(rs: regset)*) (m: mem) 
@@ -332,30 +457,30 @@ Qed.
 Lemma exec_instr_unchanged_on g f i rs m rs' m': forall
       (EI: exec_instr g f i rs m = Next rs' m'),
      Mem.unchanged_on (fun b ofs => effect_instr g (fn_code f) i rs m b ofs = false) m m'.
-Proof. intros. Admitted.
-(*    destruct i; 
+Proof. intros. 
+ destruct i;
     try solve [inv EI;
                 try solve [apply Mem.unchanged_on_refl];
                 try solve [eapply exec_load_unchanged_on; eauto];
                 try solve [eapply exec_store_unchanged_on; eauto];
-                try solve [eapply goto_label_unchanged_on; eauto]].  
-    inv EI. 
-      destruct (Val.divu (rs EAX) (rs # EDX <- Vundef r1)); inv H0.
-      destruct (Val.modu (rs EAX) (rs # EDX <- Vundef r1)); inv H1.
-      apply Mem.unchanged_on_refl.
-    inv EI.
-      destruct (Val.divs (rs EAX) (rs # EDX <- Vundef r1)); inv H0.
-      destruct (Val.mods (rs EAX) (rs # EDX <- Vundef r1)); inv H1.
-      apply Mem.unchanged_on_refl.
-    inv EI.
-      destruct (eval_testcond c0 rs); inv H0.
+                try solve [eapply goto_label_unchanged_on; eauto]].
++ (*Pdiv r1*) inv EI.
+  destruct (Val.divu (rs EAX) (rs # EDX <- Vundef r1)); inv H0.
+  destruct (Val.modu (rs EAX) (rs # EDX <- Vundef r1)); inv H1.
+  apply Mem.unchanged_on_refl.
++ (*Pidiv r1*) inv EI.
+  destruct (Val.divs (rs EAX) (rs # EDX <- Vundef r1)); inv H0.
+  destruct (Val.mods (rs EAX) (rs # EDX <- Vundef r1)); inv H1.
+  apply Mem.unchanged_on_refl.
++ (*Pcmov c rd r1*) inv EI.
+      destruct (eval_testcond c rs); inv H0.
         destruct b; inv H1; apply Mem.unchanged_on_refl.
       apply Mem.unchanged_on_refl.
-    inv EI.
-      destruct (eval_testcond c0 rs); inv H0.
++ (*Pjcc c l*) inv EI.
+      destruct (eval_testcond c rs); inv H0.
         destruct b; inv H1. eapply goto_label_unchanged_on; eauto.
       apply Mem.unchanged_on_refl.
-    inv EI.
++ (*Pjcc2 c1 c2 l*) inv EI.
       destruct (eval_testcond c1 rs); inv H0.
         destruct b; inv H1.
           destruct (eval_testcond c2 rs); inv H0.
@@ -363,11 +488,11 @@ Proof. intros. Admitted.
             apply Mem.unchanged_on_refl.
           destruct (eval_testcond c2 rs); inv H0.
             apply Mem.unchanged_on_refl.
-    inv EI.
++  (*Pjmptbl r tbl*) inv EI.
       destruct (rs r); inv H0.
         destruct (list_nth_z tbl (Int.unsigned i)); inv H1.
         eapply goto_label_unchanged_on; eauto.
-    inv EI.
++ (* Pallocframe sz ofs_ra ofs_link *) inv EI.
       remember (Mem.alloc m 0 sz) as d. 
       destruct d; apply eq_sym in Heqd; inv H0.
       remember (Mem.store Mint32 m0 b (Int.unsigned (Int.add Int.zero ofs_link)) (rs ESP)) as q.
@@ -390,7 +515,7 @@ Proof. intros. Admitted.
         rewrite PMap.gso; trivial. 
         rewrite PMap.gso; trivial. 
         eapply EmptyEffect_alloc; eassumption.
-    inv EI.
++ (* Pfreeframe sz ofs_ra ofs_link *) inv EI.
       remember (Mem.loadv Mint32 m (Val.add (rs ESP) (Vint ofs_ra))) as d.
       destruct d; inv H0.
       remember (Mem.loadv Mint32 m (Val.add (rs ESP) (Vint ofs_link))) as q.
@@ -403,32 +528,65 @@ Proof. intros. Admitted.
       Focus 2. eapply FreeEffect_free; eassumption.
       intuition. unfold effect_instr in H0.
         rewrite <- Heqw, <- Heqd, <- Heqq, Heqt in H0. trivial.
-Qed.*)
-
-(*Axiom EE1: forall g c ef res rs m b ofs,
-    effect_instr g c (Pbuiltin ef nil res) rs m b ofs = BuiltinEffect g ef nil m b ofs.
-*)
+Qed.
 
 Lemma decode_longs_nil: forall tys, decode_longs tys nil = nil.
 induction tys. trivial.  simpl in *. destruct a; trivial. Qed.
+
 Require Import msl.Extensionality.
 (*
 Lemma BuiltinEffect_decode: forall F V (ge: Genv.t F V) ef vargs,
  BuiltinEffect ge ef (decode_longs (sig_args (ef_sig ef)) vargs)=
- BuiltinEffect ge ef vargs.
-Proof. intros.
-  unfold BuiltinEffect. extensionality m. 
-  destruct ef; trivial.
+ BuiltinEffect ge ef vargs. 
+Proof. intros. (* extensionality m. extensionality bb. extensionality z.
+  remember (BuiltinEffect ge ef vargs m bb z) as RHS.
+  remember (BuiltinEffect ge ef (decode_longs (sig_args (ef_sig ef)) vargs) m bb z ) as LHS.
+  destruct RHS; destruct LHS; simpl in *; trivial. 
+  BuiltinEffect_valid_block
+  unfold BuiltinEffect. extensionality m. *)
+  destruct ef; trivial. 
   + unfold free_Effect. simpl.
     destruct vargs; simpl. reflexivity. destruct v; try reflexivity.
     destruct vargs. reflexivity.
+    extensionality m. simpl.
     destruct (Mem.load Mint32 m b (Int.unsigned i - 4)); try reflexivity.
     destruct v0; try reflexivity. 
     extensionality bb. extensionality z.
     destruct (eq_block bb b); simpl; trivial. subst.
     destruct (zlt 0 (Int.unsigned i0)); simpl; trivial.
     destruct (zle (Int.unsigned i - 4) z ); simpl; trivial.
-    destruct (zlt z (Int.unsigned i + Int.unsigned i0)); simpl; trivial. omega.
+    destruct (zlt z (Int.unsigned i + Int.unsigned i0)); simpl; trivial. admit. (*2.6?*)
+  + extensionality m. extensionality bb. extensionality z.
+    remember (BuiltinEffect ge (EF_memcpy sz al) vargs m bb z) as r.
+    remember (BuiltinEffect ge (EF_memcpy sz al) (decode_longs (sig_args (ef_sig (EF_memcpy sz al))) vargs) m bb z) as l.
+    symmetry in Heql; symmetry in Heqr.
+    destruct r.
+    - specialize (BuiltinEffect_valid_block _ _ _ _ _ _ Heqr); intros.
+      destruct Heql;  simpl in *; trivial.
+      destruct vargs; simpl in *; try discriminate.
+      destruct v; simpl in *; try discriminate. 
+      destruct vargs; simpl in *; try discriminate.
+      destruct v; simpl in *; try discriminate.
+      destruct vargs; simpl in *; try discriminate. trivial.
+    - destruct l; trivial. specialize (BuiltinEffect_valid_block _ _ _ _ _ _ Heql); intros.
+      simpl in *. 
+      destruct vargs; simpl in *; try discriminate.
+      destruct v; simpl in *; try discriminate. 
+      destruct vargs; simpl in *; try discriminate.
+      destruct v; simpl in *; try discriminate.
+      destruct vargs; simpl in *; try discriminate. rewrite Heqr in Heql. discriminate.
+ trivial.
+    destruct vargs. reflexivity. destruct v; try reflexivity.
+    destruct vargs. reflexivity.
+    extensionality m; simpl. extensionality bb. extensionality z.
+    destruct (eq_block bb b); simpl; trivial. subst.
+    destruct (zle (Int.unsigned i) z); simpl; trivial.
+    destruct (zle 0 sz); simpl; trivial.
+    destruct (zlt z (Int.unsigned i +sz)); simpl; trivial.
+    specialize (Int.unsigned_range i). intros [? _]. omega.
+    SearchAbout Int.unsigned. omega.
+    destruct (zlt z (Int.unsigned i + Int.unsigned i0)); simpl; trivial. admit. (*TODO 2.6???*)
+  + unfold memcpy_Effect. simpl.
 Qed.
 
  BuiltinEffect ge ef (map tls (loc_arguments (ef_sig ef))) =
@@ -439,20 +597,20 @@ Proof. intros.
   destruct ef; trivial.
 Qed.
 *)
-Lemma asmstep_effax1: forall (M : block -> Z -> bool) g c m c' m',
+Lemma asmstep_effax1: forall (M : block -> Z -> bool) g c m c' m'
+      (HF: helper_functions_declared g hf),
       asm_effstep g M c m c' m' ->
-      (asm_step (*hf*) g c m c' m' /\
+      (asm_step hf g c m c' m' /\
        Mem.unchanged_on (fun (b : block) (ofs : Z) => M b ofs = false) m m').
-Proof. Admitted.
- (*Proof.
+Proof. 
 intros.
-destruct H.
-+ split. eapply asm_exec_step_internal; eassumption.
+destruct H. 
++ split. eapply asm_exec_step_internal; eassumption. 
   clear -H2 hf. eapply exec_instr_unchanged_on; eassumption.
-+ split. eapply asm_exec_step_builtin; eassumption.
-  simpl. Locate BuiltinEffect_decode. in H6. subst. eapply BuiltinEffect_unchOn. eassumption. eassumption. inv H2.
++ split. eapply asm_exec_step_builtin; try eassumption. admit. (*~ isInlinedAssembly ef*)
+  simpl. subst E. inv H2. (*   eapply BuiltinEffect_unchOn. eassumption. eassumption. eassumption. inv H2.*)
   - rewrite decode_longs_nil. eapply BuiltinEffect_unchOn; eassumption.
-  - eapply BuiltinEffect_unchOn. eassumption. eassumption. 
+  - rewrite <- BuiltinEffect_decode. simpl. eapply BuiltinEffect_unchOn. eassumption. eassumption. eassumption.
   assert (EE1: effect_instr g (fn_code f) (Pbuiltin ef nil res) rs m b0 ofs0 = BuiltinEffect g ef nil m b0 ofs0).
          eapply BuiltinEffect_unchOn; eassumption. 
   admit. (*
